Linglib/Logic/Modal/BSML/ClassicalValidities.lean
@@ -51,7 +51,7 @@ namespace BSML
 
 open ModalLogic (KripkeModel)
 
-variable {W : Type*} [DecidableEq W] [Fintype W] {Atom : Type*}
+variable {W : Type*} [DecidableEq W] {Atom : Type*}
 
 /-! ### Box-diamond duality -/
 
